Wellformedness.v
@@ -1,0 +1,62 @@
+From Celsius Require Export Trees.
+From Celsius Require Export Eval.
+From Celsius Require Export PartialMonotonicity.
+From Celsius Require Export Reachability.
+From Celsius Require Export Compatibility.
+Require Import ssreflect ssrbool.
+
+Require Import List.
+Import ListNotations.
+Open Scope nat_scope.
+Require Import Sets.Ensembles.
+
+(*
+  Notation "σ ⊨ l1 ⇝ l2" := (σ + l1 + l2) (at level 80, l1 at level 80, l2 at level 80).
+  Notation "σ1 ⇝ σ2 ⋖ L" := (σ1 * σ2 * L) (at level 81, σ2 at level 81).
+  Eval compute in (2 ⊨ 2 ⇝ 3) + (1 ⇝ 2 ⋖ 3).
+  Check (1 ⊨ 2 ⇝ 3).
+  Check (2 ⇝ 3 ⋖ 4).
+ *)
+
+Module Wellformedness.
+  Import Eval.Evaluator.
+
+  Definition wf σ := forall l C ω, getObj σ l = Some(C,ω) -> forall f l, getVal ω f = Some l -> l < dom σ.
+
+  Definition storeSubset (σ: Store) L := (forall l, (l ∈ L) -> l < (dom σ)).
+  Notation "L ⪽ σ" := (storeSubset σ L) (at level 80).
+  Definition codom (ρ: Env) : (LocSet):=
+    fun (l: Loc) => (List.In l ρ).
+
+  Notation " a ∪ { b } " := (Union Loc a (Singleton Loc b)) (at level 80).
+  Lemma storeSubset_singleton : forall a b σ, a ∪ {b} ⪽ σ -> b < dom σ.
+  Proof.
+    intros. apply (H b).
+    eauto using Union_intror, In_singleton.
+  Qed.
+
+
+  Theorem wellformedness_conserved :
+    forall k e σ σ' ρ ψ l, ⟦e⟧(σ, ρ, ψ)(k) = (Success l σ') -> wf σ -> (codom ρ) ∪ {ψ} ⪽ σ -> (wf σ' /\ l < dom σ').
+    apply (strong_induction (fun k => forall e σ σ' ρ ψ l, ⟦e⟧(σ, ρ, ψ)(k) = (Success l σ') -> wf σ -> (codom ρ) ∪ {ψ} ⪽ σ ->  (wf σ' /\ l < dom σ'))). intros.
+    assert (ψ < dom σ /\ forall l', List.In l' ρ -> l' < dom σ). {
+      unfold storeSubset in *.
+      split; steps; eauto using Union_introl, Union_intror, In_singleton. }
+    destruct_and.
+    destruct n => //.
+    move : (PeanoNat.Nat.lt_succ_diag_r n) => Hn.
+    destruct e ;
+      repeat light || invert_constructor_equalities || destruct_match ||
+             match goal with
+             | H1 : ⟦ _ ⟧ ( _, _, _)( _ ) = Success _ _ |- _ =>
+               pose proof (H n Hn _ _ _ _ _ _ H1); clear H1 end ||
+             eauto 3 using nth_error_In.
+    unfold wf in H5. eapply H5; eauto.
+    destruct l1 => //. destruct l0, n => //. simpl in *. invert_constructor_equalities; subst.  apply H5 => //.
+    intros l' Hl'. induction Hl' => //. induction H0. admit.
+    simpl in *.
+    admit.
+  Admitted.
+
+
+End Wellformedness.
